SetTheory/Basic.lean
@@ -1,36 +1,164 @@
-import Aesop
-
-/-!
-# Models of set theory
--/
-
-/-- M is a *model of set theory* if it has a membership operation.
-Elements of M are called *classes*. -/
-class SetTheory (M : Type _) extends Membership M M
+import SetTheory.Axioms
 
 namespace SetTheory
 
-instance [SetTheory M] : HasSubset M where
-  Subset x y := ∀ ⦃z : M⦄, z ∈ x → z ∈ y
+variable [MorseKelley M] {x y z : M}
 
-@[aesop unsafe 50% apply]
-theorem subset_iff [SetTheory M] (x y : M) : x ⊆ y ↔ ∀ ⦃z : M⦄, z ∈ x → z ∈ y :=
-  Iff.rfl
+theorem left_mem_pair : IsSet x → IsSet y → x ∈ pair x y :=
+  by aesop
 
-/-- A class is a *set* if it is an element of a class. -/
-def IsSet [SetTheory M] (x : M) : Prop :=
-  ∃ y : M, x ∈ y
+theorem right_mem_pair : IsSet x → IsSet y → x ∈ pair x y :=
+  by aesop
 
-theorem isSet_of_mem [SetTheory M] {x y : M} (h : x ∈ y) : IsSet x :=
-  ⟨y, h⟩
+@[simp]
+theorem pair_self : pair x x = {x} :=
+  rfl
 
-/-- A *set* in a set theory M is a class that is a set.
-Not to be confused with Mathlib's `Set`. -/
-def Set (M : Type _) [SetTheory M] : Type _ :=
-  {x : M // IsSet x}
+@[aesop safe]
+theorem pair_nonemptyClass : IsSet x → IsSet y → NonemptyClass (pair x y) :=
+  fun hx hy => ⟨x, left_mem_pair hx hy⟩
 
-/-- A class is *nonempty* if it has an element. -/
-def NonemptyClass [SetTheory M] (x : M) : Prop :=
-  ∃ y : M, y ∈ x
+/-- The intersection of a set `x`. Constructed as the class `{y | ∀ t, t ∈ x → y ∈ t}`. -/
+def sInter (x : M) : M :=
+  ofFormula (.all (.imp
+    (.mem (Sum.inr 1) (Sum.inl ()))
+    (.mem (Sum.inr 0) (Sum.inr 1))))
+  (fun (_ : Unit) => x)
+
+/-- We will use the notation `⋂` for set intersection in this project. -/
+prefix:110 "⋂ " => sInter
+
+@[aesop norm]
+theorem mem_sInter_iff (hx : NonemptyClass x) :
+    y ∈ ⋂ x ↔ ∀ t ∈ x, y ∈ t := by
+  unfold sInter
+  simp
+  intro h
+  obtain ⟨z, hz⟩ := hx
+  exact ⟨z, h z hz⟩
+
+theorem subset_sInter : NonemptyClass x → y ∈ x → ⋂ x ⊆ y := by
+  intro hx h z hz
+  aesop
+
+theorem sInter_isSet (hx : NonemptyClass x) : IsSet (⋂ x) := by
+  obtain ⟨y, hy⟩ := hx
+  refine subset_isSet (subset_sInter ⟨y, hy⟩ hy) ⟨x, hy⟩
+
+/-- The intersection of two sets `x` and `y`. -/
+instance : Inter M where
+  inter x y := sInter (pair x y)
+
+@[simp]
+theorem mem_inter_iff (hx : IsSet x) (hy : IsSet y) :
+    z ∈ x ∩ y ↔ z ∈ x ∧ z ∈ y := by
+  show z ∈ sInter (pair x y) ↔ z ∈ x ∧ z ∈ y
+  rw [mem_sInter_iff (pair_nonemptyClass hx hy)]
+  aesop
+
+@[simp]
+theorem sUnion_pair : ⋃ pair x y = x ∪ y := rfl
+
+@[simp]
+theorem sInter_pair : ⋂ pair x y = x ∩ y := rfl
+
+/-- The axiom scheme of *separation*. -/
+def sep (p : BoundedFormula α 1) (v : α → M) (x : M) : M :=
+  ofFormula (
+    (p.sum Unit).and
+    (.mem (Sum.inr 0) (Sum.inl (Sum.inr ()))))
+  (Sum.elim v (fun _ => x))
+
+@[simp]
+theorem mem_sep_iff : x ∈ sep p v y ↔ x ∈ y ∧ Interpret M p v (fun _ => x) := by
+  unfold sep
+  aesop
+
+@[simp]
+theorem union_self (hx : IsSet x) : x ∪ x = x :=
+  by ext; aesop
+
+@[simp]
+theorem inter_self (hx : IsSet x) : x ∩ x = x :=
+  by ext; aesop
+
+theorem union_pair_eq_inter_pair (hx : IsSet x) (hy : IsSet y) :
+    {x} ∪ pair x y = {x} ∩ pair x y ↔ x = y := by
+  constructor
+  · intro h
+    rw [ext_iff] at h
+    have := (h y).mp ?_
+    · rw [mem_inter_iff (singleton_isSet hx) (pair_isSet hx hy),
+        mem_singleton_iff hx] at this
+      exact this.1.symm
+    · rw [mem_union_iff (singleton_isSet hx) (pair_isSet hx hy)]
+      aesop
+  · rintro rfl
+    simp [union_self (singleton_isSet hx), inter_self (singleton_isSet hx)]
+
+/-- The first projection of a Kuratowski ordered pair. -/
+def π₁ (x : M) : M :=
+  ⋃ ⋂ x
+
+/-- The second projection of a Kuratowski ordered pair. -/
+def π₂ (x : M) : M :=
+  ⋃ sep
+    (.imp
+      (.ne (Sum.inl true) (Sum.inl false))
+      (.not (.mem (Sum.inr 0) (Sum.inl false))))
+    (fun i => if i then ⋃ x else ⋂ x) (⋃ x)
+
+theorem mem_π₂_iff : y ∈ π₂ x ↔ ∃ z, y ∈ z ∧ z ∈ ⋃ x ∧ (⋃ x ≠ ⋂ x → z ∉ ⋂ x) := by
+  unfold π₂
+  aesop
+
+@[simp]
+theorem π₁_opair (hx : IsSet x) (hy : IsSet y) : π₁ (opair x y) = x := by
+  unfold π₁ opair
+  ext z
+  simp [mem_inter_iff (singleton_isSet hx) (pair_isSet hx hy)]
+  aesop
+
+@[simp]
+theorem π₂_opair (hx : IsSet x) (hy : IsSet y) : π₂ (opair x y) = y := by
+  unfold opair
+  ext z
+  rw [mem_π₂_iff]
+  simp only [sUnion_pair, sInter_pair, ne_eq, union_pair_eq_inter_pair hx hy]
+  constructor
+  · rintro ⟨s, hzs, hsx, hs⟩
+    by_cases h : s = y
+    · subst h
+      exact hzs
+    rw [mem_union_iff (singleton_isSet hx) (pair_isSet hx hy),
+      mem_singleton_iff hx] at hsx
+    cases hsx with
+    | inl hsx =>
+      subst hsx
+      exfalso
+      refine hs h ?_
+      rw [mem_inter_iff (singleton_isSet hx) (pair_isSet hx hy)]
+      aesop
+    | inr hsx =>
+      rw [mem_pair_iff hx hy] at hsx
+      cases hsx with
+      | inl hsx =>
+        subst hsx
+        exfalso
+        refine hs h ?_
+        rw [mem_inter_iff (singleton_isSet hx) (pair_isSet hx hy)]
+        aesop
+      | inr hsx =>
+        subst hsx
+        exact hzs
+  · intro hzy
+    refine ⟨y, hzy, ?_, ?_⟩
+    · rw [mem_union_iff (singleton_isSet hx) (pair_isSet hx hy),
+        mem_pair_iff hx hy]
+      exact Or.inr (Or.inr rfl)
+    · intro h
+      refine (fun h' => h ?_)
+      rw [mem_inter_iff (singleton_isSet hx) (pair_isSet hx hy)] at h'
+      aesop
 
 end SetTheory
