SetTheory.lean
@@ -1,3 +1,4 @@
-import SetTheory.Basic
+import SetTheory.SetTheory
 import SetTheory.Formula
 import SetTheory.Axioms
+import SetTheory.Basic
